---
title: "Fourier transforms"
---

::: {.hidden}
 \providecommand{\vv}[1]{{\mathbf{#1}}}
 \providecommand{\pd}[2]{{\frac{\partial #1}{\partial #2}}}
:::

Fourier series work great when we have a function which is perfectly periodic, or defined on a finite interval. But often in practice we have functions defined on the whole real line, when we use an approximation that something in infinitely big.

In this case, there isn't an exact wavelength that fits perfectly, and instead we have to consider all possible wavelengths. This leads us to the _Fourier transform_.

## Definition of the Fourier transform
The _Fourier transform_ of a function $f(x)$ is defined as^[Lots of different conventions exist for the Fourier transform, this is one of the most common.]
$$
F(k) = \frac{1}{\sqrt{2\pi}}\int_{-\infty}^\infty f(x) e^{-ikx}\,dx,
$$
where $k$ is called the _wave number_.

The _inverse Fourier transform_ is given by
$$
f(x) = \frac{1}{\sqrt{2\pi}}\int_{-\infty}^\infty F(k) e^{ikx}\,dk.
$$
These two equations are very similar in form to the Fourier series equations, but now we have integrals over all possible wave numbers $k$ instead of sums over discrete wavelengths.

## Example
Find the Fourier transform of
$$
f(x) = e^{-\frac{x^2}{2}}.
$$

::: {.callout-tip collapse="true"}
## Solution
We have
$$
F(k) = \frac{1}{\sqrt{2\pi}}\int_{-\infty}^\infty e^{-\frac{x^2}{2}} e^{-ikx}\,dx.
$$
Combining the exponents gives
$$
F(k) = \frac{1}{\sqrt{2\pi}}\int_{-\infty}^\infty e^{-\frac{x^2}{2} - ikx}\,dx = \frac{1}{\sqrt{2\pi}}\int_{-\infty}^\infty e^{-\frac{x^2 + 2ikx}{2}}\,dx.
$$
Completing the square in the exponent:
$$
x^2 + 2ikx = (x + ik)^2 - k^2,
$$
so
$$
F(k) = \frac{1}{\sqrt{2\pi}}\int_{-\infty}^\infty e^{-\frac{(x + ik)^2 - k^2}{2}}\,dx = \frac{e^{\frac{k^2}{2}}}{\sqrt{2\pi}}\int_{-\infty}^\infty e^{-\frac{(x + ik)^2}{2}}\,dx.
$$
Now we can make the substitution $u = x + ik$, so $du = dx$. The limits of integration remain $-\infty$ to $\infty$ since shifting by a constant (even a complex one) doesn't change them. Thus,
$$
F(k) = \frac{e^{\frac{k^2}{2}}}{\sqrt{2\pi}}\int_{-\infty}^\infty e^{-\frac{u^2}{2}}\,du.
$$
The integral is just the standard Gaussian integral, which evaluates to $\sqrt{2\pi}$. Therefore,
$$
F(k) = \frac{e^{\frac{k^2}{2}}}{\sqrt{2\pi}} \cdot \sqrt{2\pi} = e^{\frac{k^2}{2}}.
$$
So the Fourier transform of $f(x) = e^{-\frac{x^2}{2
}}$ is
$$
F(k) = e^{\frac{k^2}{2}}.
$$
:::